Added more comments and description

boogie/sv_boogie.bpl
@@ -1,12 +1,29 @@
-// Introduce a constant 'N' and postulate that it is non-negative
-// TODO: should we make N var instead of const?
-// or use the bucket sort individual length as parameter for quicksort?
 const N: int;
-axiom 0 <= N;
+// TODO why this? and not 1 <= N?
+axiom 10 <= N;
 
-// Declare a map from integers to integers.
-// 'a' should be treated as an array of 'N' elements, indexed from 0 to N-1
-var a: [int]int;
+var a, old_a, perm: [int]int;
+
+function vi(i: int): bool
+{
+  0 <= i && i < N
+}
+
+function perm(a: [int]int): bool
+{
+  // WARNING: doesn't work with:
+  // (forall i: int :: vi(i) ==> vi(a[i]))
+  (forall i: int :: vi(i) ==> 0 <= a[i] && a[i] < N)
+  &&
+  (forall i, j: int :: 0 <= i && i < j && j < N ==> a[i] != a[j])
+}
+
+function perm_of(a, b, perm: [int]int): bool
+{
+  perm(perm)
+  &&
+  (forall i: int :: vi(i) ==> a[i] == b[perm[i]])
+}
 
 // Returns true iff the elements of 'arr' are small (i.e. values in the range -3N to +3N)
 function has_small_elements(arr: [int]int): bool
@@ -14,146 +31,254 @@ function has_small_elements(arr: [int]int): bool
   (forall i: int :: (0 <= i && i < N) ==> (-3 * N <= arr[i] && arr[i] <= 3 * N))
 }
 
-// Recursive implementation of quicksort
-procedure quicksort(lo: int, hi: int) returns ()
-  modifies a;
+// Returns true iff the elements from a[lo] to a[hi] are sorted
+function sorted(a: [int]int, lo, up: int): bool
 {
-  var p: int;
-  if (lo < hi) {
-    call p :=  partition(lo, hi);
-    call quicksort(lo, p-1);
-    call quicksort(p+1, lo);
-  }
-}
-// helper function for quicksort to partition the array
-procedure partition(lo:int, hi: int) returns (p: int)
-  requires 0 <= lo && hi <= N;
-  modifies a;
-  ensures lo <= p && hi > p;
-  ensures (forall k: int, j: int :: lo <= k && k < p && p <= j && j < hi  ==>  a[k] <= a[j]);
-  ensures (forall k: int :: lo <= k && k < p  ==>  a[k] <= old(a)[lo]);
-  ensures (forall k: int :: p <= k && k < hi  ==>  old(a)[lo] <= a[k]);
-{
-  var pivot, i,j,temp: int;
-  pivot := a[hi];
-  i := lo;
-  j := lo;
-  while(j <= hi-1) {
-    if(a[j] <= pivot) {
-      // swap
-      call swap(i,j);
-      i := i+1;
-    }
-  }
-  call swap(i, hi);
-  p := i;
-  return;
+  (forall i, j: int :: lo <= i && i <= j && j <= up ==> a[i] <= a[j])
 }
 
-// swap arr[a] with arr[b]
-procedure swap(x:int, y:int) returns ()
-  requires 0 <= x && y <= N;
-  modifies a;
-  ensures a[x] == old(a)[y] && a[y] == old(a)[x];
+
+procedure init()
+  modifies a, perm;
+  ensures perm_of(a, old_a, perm);
+{
+  var k: int;
+  k := 0;
+  while (k < N)
+  {
+    a[k] := old_a[k];
+    perm[k] := k;
+  }
+}
+/*
+  swaps content of a at locations i and j
+*/
+procedure swap(i, j: int)
+  requires perm_of(a, old_a, perm);
+  requires vi(i);
+  requires vi(j);
+  modifies a, perm;
+  ensures a[i] == old(a)[j];
+  ensures a[j] == old(a)[i];
+  ensures perm_of(a, old_a, perm);
+  // we do not touch anything other than the values a[j] and a[i]
+  ensures (forall k: int :: k != i && k != j ==> a[k] == old(a)[k]);
 {
   var temp: int;
-  temp := a[x];
-  a[x] := a[y];
-  a[y] := temp;
+
+  temp := perm[i];
+  perm[i] := perm[j];
+  perm[j] := temp;
+
+  temp := a[i];
+  a[i] := a[j];
+  a[j] := temp;
 }
 
-// bucket sort implementation using 3 buckets
-procedure bucketsort(N: int) returns ()
+/*
+  partitions a between lo and hi into two parts
+  one part with all values below the pivot
+  another part with all values above the pivot
+  Returns: index p which divides a in
+           a) elements greater equal pivot
+           b) elements smaller pivot
+           p is the index of the first element in a
+*/
+procedure partition(lo, hi, pivot: int) returns (p: int)
+  requires 0 <= lo && lo <= hi && hi < N;
+  requires perm_of(a, old_a, perm);
+  modifies a, perm;
+  ensures perm_of(a, old_a, perm);
+  ensures lo <= p && p <= hi + 1;
+  // all values from lo to p are smaller than the pivot
+  ensures (forall k: int :: lo <= k && k < p ==> a[k] < pivot);
+  // all values from p to hi are greater-equal the pivot
+  ensures (forall k: int :: p <= k && k <= hi ==> pivot <= a[k]);
+  // we don't touch the array outside lo and hi
+  ensures (forall k: int :: k < lo ==> a[k] == old(a)[k]);
+  ensures (forall k: int :: hi < k ==> a[k] == old(a)[k]);
+  // all values between lo and hi are greater-equal all values below lo
+  ensures (forall i: int :: i < lo ==>
+    (forall k: int :: lo <= k && k <= hi ==> old(a)[i] <= old(a)[k])
+    ==> (forall k: int :: lo <= k && k <= hi ==> a[i] <= a[k])
+  );
+  // all values between lo and hi are smaller all values above hi
+  ensures (forall i: int :: hi < i ==>
+    (forall k: int :: lo <= k && k <= hi ==> old(a)[k] <= old(a)[i])
+    ==> (forall k: int :: lo <= k && k <= hi ==> a[k] <= a[i])
+  );
+{
+  var i, j: int;
+
+  i := lo;
+  j := hi;
+
+  while (i < j)
+   invariant lo <= i && i <= j && j <= hi;
+   invariant perm_of(a, old_a, perm);
+   invariant (forall k: int :: lo <= k && k < i ==> a[k] < pivot);
+   invariant (forall k: int :: j < k && k <= hi ==> pivot <= a[k]);
+   invariant (forall k: int :: i < k && k < j ==> a[k] == old(a)[k]);
+   invariant (forall k: int :: k < lo ==> a[k] == old(a)[k]);
+   invariant (forall k: int :: hi < k ==> a[k] == old(a)[k]);
+   invariant (forall l: int :: l < lo ==>
+    (forall k: int :: lo <= k && k <= hi ==> old(a)[l] <= old(a)[k])
+    ==> (forall k: int :: lo <= k && k <= hi ==> a[l] <= a[k])
+   );
+   invariant (forall l: int :: hi < l ==>
+    (forall k: int :: lo <= k && k <= hi ==> old(a)[k] <= old(a)[l])
+    ==> (forall k: int :: lo <= k && k <= hi ==> a[k] <= a[l])
+   );
+  {
+    while (a[i] < pivot && i < j)
+      invariant lo <= i && i <= j && j <= hi;
+      invariant (forall k: int :: lo <= k && k < i ==> a[k] < pivot);
+    {
+      i := i + 1;
+    }
+
+    if (i == j) {
+      break;
+    }
+
+    while (pivot <= a[j] && i < j)
+      invariant lo <= i && i <= j && j <= hi;
+      invariant (forall k: int :: j < k && k <= hi ==> pivot <= a[k]);
+    {
+      j := j - 1;
+    }
+
+    if (i == j) {
+      break;
+    }
+
+    call swap(i, j);
+  }
+
+  if (a[i] < pivot) {
+    i := i + 1;
+  }
+
+  p := i;
+}
+
+/*
+  sorts a from indices lo to hi using quicksort
+*/
+procedure quicksort(lo, hi: int)
+  requires 0 <= lo;
+  requires lo <= hi;
+  requires hi < N;
+  requires perm_of(a, old_a, perm);
+  modifies a, perm;
+  // a is a permutation of the old a
+  ensures perm_of(a, old_a, perm);
+  // a from lo to hi is sorted
+  ensures sorted(a, lo, hi);
+  // we don't modify anything below lo
+  ensures (forall k: int :: k < lo ==> a[k] == old(a)[k]);
+  // we don't modify anything above hi
+  ensures (forall k: int :: hi < k ==> a[k] == old(a)[k]);
+  // every element in a between lo and high is larger than a[lo-1] (the largest element before lo)
+  ensures (forall k,i: int :: lo <= k && k <= hi ==> old(a)[lo - 1] <= old(a)[k])
+       ==> (forall k: int :: lo <= k && k <= hi ==> a[lo - 1] <= a[k]);
+  // every element in a between lo and high is smaller than a[hi+1] (the smallest element after hi)
+  ensures (forall k: int :: lo <= k && k <= hi ==> old(a)[k] <= old(a)[hi + 1])
+       ==> (forall k: int :: lo <= k && k <= hi ==> a[k] <= a[hi + 1]);
+{
+  var p: int;
+
+  if (lo == hi) {
+    return;
+  } else if (lo + 1 == hi) {
+    if (a[lo] > a[hi]) {
+      call swap(lo, hi);
+    }
+    return;
+  }
+
+  call p := partition(lo, hi - 1, a[hi]);
+
+  call swap(p, hi);
+
+  if (lo < p) {
+    call quicksort(lo, p - 1);
+  }
+  if (p < hi) {
+    call quicksort(p + 1, hi);
+  }
+}
+
+/*
+  sorts a using bucketsort
+*/
+procedure bucketsort()
+  requires perm_of(a, old_a, perm);
+  // TODO: not sure if we need this, but won't hurt
   requires has_small_elements(a);
-  modifies a;
+  modifies a, perm;
+  ensures perm_of(a, old_a, perm);
+  ensures sorted(a, 0, N - 1);
 {
-  // model buckets as three different integer maps
-  // this is fine according to the FAQ
-  var bucket1, bucket2, bucket3: [int]int;
-  var size1, size2, size3: int;
-  // backup a and n to be able to use it for quicksort
-  var old_a: [int]int;
-  var old_N,i: int;
+  /*
+   * Choose buckets such that each bucket's range is
+   * [-3*N, -N), [-N, N) & [N, 3*N] resp.
+   *
+   * Furthermore choose b1 & b2 such that each bucket's indices is in
+   * [0, b1), [b1, b2), [b2, N] resp.
+   */
+  var b1, b2: int;
 
-  size1 := 0;
-  size2 := 0;
-  size3 := 0;
+  // do first bucket
+  call b1 := partition(0, N - 1, -N);
 
-  old_a := a;
-  old_N := N;
-  //N := xxx;
-  // TODO: what should we do with N? See line 2
-  i := 0;
-  while(i < N)
-  {
-    if(a[i] < -N)
-    {
-      bucket1[i] := a[i];
-      size1 := size1+1;
-    }
-    if(a[i] >= -N && a[i] < N)
-    {
-      bucket2[i] := a[i];
-      size2 := size2+1;
-    }
-    if(a[i] >= N)
-    {
-      bucket3[i] := a[i];
-      size3 := size3+1;
-    }
-    i := i+1;
-  }
-  a := bucket1;
-  call quicksort(0,size1-1);
-  bucket1 := a;
-  a := bucket2;
-  call quicksort(0,size2-1);
-  bucket2 := a;
-  a := bucket3;
-  call quicksort(0,size3-1);
-  bucket3 := a;
-  call bucketmerge(bucket1, bucket2, bucket3, size1, size2, size3);
-}
+  assert b1 <= N;
 
-// helper function to merge the 3 buckets
-procedure bucketmerge(bucket1: [int]int, bucket2: [int]int, bucket3: [int]int, size1: int, size2: int, size3: int) returns ()
-  modifies a;
-{
-  var counter,i : int;
-  counter := 0;
-  i :=0;
-  while(i < size1)
-  {
-    a[counter+i] := bucket1[i];
-    i := i+1;
+  // return with a single quicksort immediately if b1 is
+  // outside the range [0,N-1]
+  if (b1 == N) {
+    call quicksort(0, b1 - 1);
+    return;
   }
-  counter := i;
-  i := 0;
-  while(i < size2)
-  {
-    a[counter+i] := bucket2[i];
-    i := i+1;
+
+  if (0 < b1) {
+    assert (forall k: int :: 0 <= k && k < b1 ==> a[k] < a[b1]);
+    call quicksort(0, b1 - 1);
+    // should probably generalize the semantics that establish
+    // in partition & quicksort that the respective blocks don't change their
+    // relationship to upper and lower limits.
+    assert (forall k: int :: 0 <= k && k < b1 ==> a[k] < a[b1]);
   }
-  counter := i;
-  i := 0;
-  while(i < size3)
-  {
-    a[counter+i] := bucket3[i];
-    i := i+1;
+
+  //assert -N <= a[b1];
+  //assert (forall k: int :: 0 <= k && k < b1 ==> a[k] < -N);
+  assert (forall k: int :: 0 <= k && k < b1 ==> a[k] < a[b1]);
+
+  // do second and third bucket
+  call b2 := partition(b1, N - 1, N);
+
+  if (b1 < b2) {
+    call quicksort(b1, b2 - 1);
   }
+  assert sorted(a, 0, b2 - 1);
+  if (b2 < N) {
+    call quicksort(b2, N - 1);
+  }
+  assert sorted(a, 0, N - 1);
 }
 
 // Sorts 'a' using bucket sort or quick sort, as determined by has_small_elements(a)
 procedure sort() returns ()
-  modifies a;
+  modifies a, perm;
+  ensures perm_of(a, old_a, perm);
+  ensures sorted(a, 0, N - 1);
 {
+  call init();
   if (has_small_elements(a))
   {
-      // sort 'a' using bucket sort
-      call bucketsort(N);
+    call bucketsort();
   } else
   {
-      // sort 'a' using quick sort
-      call quicksort(0, N-1);
+    call quicksort(0, N - 1);
   }
 }
